证明:
$$
\varphi_{n+1}(x)=(x-\alpha_{n})\varphi_{n}(x)-\beta_{n}\varphi_{n-1}(x)
$$
其中 $\varphi_{0}=1,\varphi_{1}=x,\alpha_{n}=\frac{(x\varphi_{n},\varphi_n)}{(\varphi_{n},\varphi_{n)}},\beta_{n}=\frac{(\varphi_{n},\varphi_{n})}{(\varphi_{n-1},\varphi_{n-1})}$

证:
通过多项式除法可知
$$
\varphi_{n+1}=x\varphi_{n}+\sum\limits_{i=0}^{n}\alpha_{i}\varphi_{i}\tag{1}
$$
即:
$$
x\varphi_{n}=\varphi_{n+1}-\sum\limits_{i=0}^{n}\alpha_{i}\varphi_{i}\tag{2}
$$
根据正交多项式的性质 $(\varphi_{n+1},\varphi_{k})=0,n+1\neq k$ 可得 
$$
(\varphi_{n+1},\varphi_{k})=(x\varphi_{n}+\sum\limits_{i=0}^{n}\alpha_{i}\varphi_{i},\varphi_{k})=(x\varphi_{n},\varphi_{k})+\sum\limits_{i=0}^{n}\alpha_{i}(\varphi_{i},\varphi_{k})=0\tag{3}
$$
当 k=n 时, 由 (3) 有 $(x\varphi_{n},\varphi_{n})+\alpha_{n}(\varphi_{n},\varphi_{n})=0$
可得
$$
\alpha_{n}=-\frac{(x\varphi_{n},\varphi_{n})}{(\varphi_{n},\varphi_{n})}\tag{4}
$$
当 k=n-1 时, 由 (2), (3) 同理有 $(\varphi_{n},\varphi_{n})+\alpha_{n-1}(\varphi_{n-1},\varphi_{n-1})=0$
可得
$$
\alpha_{n-1}=-\frac{(\varphi_{n},\varphi_{n})}{(\varphi_{n-1},\varphi_{n-1})}\tag{5}
$$
当 k<n-1 时, 由 (2), (3) 同理可得
$$
\alpha_{k}=0\tag{6}
$$
将 (4), (5), (6) 带入 (1) 得 
$$
\varphi_{n+1}(x)=(x-\alpha_{n})\varphi_{n}(x)-\beta_{n}\varphi_{n-1}(x)
$$
其中 $\varphi_{0}=1,\varphi_{1}=x,\alpha_{n}=\frac{(x\varphi_{n},\varphi_n)}{(\varphi_{n},\varphi_{n)}},\beta_{n}=\frac{(\varphi_{n},\varphi_{n})}{(\varphi_{n-1},\varphi_{n-1})}$
原式得证